Iris/Iris/Algebra/IsOp.lean
@@ -24,7 +24,7 @@ section IsOp
 @[ipm_class, rocq_alias IsOp, rocq_alias IsOp', rocq_alias IsOp'LR]
 class IsOp [CMRA α]
     (io : InOut) (a : semiOutParamIPM io α)
-    (b1 : semiOutParamIPM io α true) (b2 : semiOutParamIPM io α true) where
+    (b1 : semiOutParamIPM io.negate α) (b2 : semiOutParamIPM io.negate α) where
   is_op : a ≡ b1 • b2
 
 /--
