Iris/Iris/ProofMode/Instances.lean
@@ -19,27 +19,27 @@ open Iris.BI Iris.Std
 -- AsEmpValid
 @[rocq_alias as_emp_valid_emp_valid]
 instance (priority := default + 10) asEmpValidEmpValid
-    [bi : BI PROP] d (P : PROP) :
-    AsEmpValid d (⊢ P) io PROP bi P := ⟨by simp⟩
+    [bi : BI PROP] d (P : PROP) : AsEmpValid d (⊢ P) PROP bi P where
+  as_emp_valid := by simp
 
 @[rocq_alias as_emp_valid_entails]
-instance asEmpValid_entails [bi : BI PROP] d (P Q : PROP)
-: AsEmpValid d (P ⊢ Q) io PROP bi iprop(P -∗ Q) where
+instance asEmpValid_entails [bi : BI PROP] d (P Q : PROP) :
+    AsEmpValid d (P ⊢ Q) PROP bi iprop(P -∗ Q) where
   as_emp_valid := ⟨λ _ => entails_wand, λ _ => wand_entails⟩
 
-instance asEmpValid_bientails [bi : BI PROP] (P Q : PROP)
-: AsEmpValid d (P ⊣⊢ Q) io PROP bi iprop(P ∗-∗ Q) where
+instance asEmpValid_bientails [bi : BI PROP] (P Q : PROP) :
+    AsEmpValid d (P ⊣⊢ Q) PROP bi iprop(P ∗-∗ Q) where
   as_emp_valid := ⟨λ _ => equiv_wandIff, λ _ => wandIff_equiv⟩
 
 @[rocq_alias as_emp_valid_equiv]
-instance asEmpValid_equiv [bi : BI PROP] (P Q : PROP)
-: AsEmpValid d (P ≡ Q) io PROP bi iprop(P ∗-∗ Q) where
+instance asEmpValid_equiv [bi : BI PROP] (P Q : PROP) :
+    AsEmpValid d (P ≡ Q) PROP bi iprop(P ∗-∗ Q) where
   as_emp_valid := ⟨λ _ h => equiv_wandIff (equiv_iff.1 h), λ _ h => (equiv_iff.2 (wandIff_equiv h))⟩
 
 @[rocq_alias as_emp_valid_forall]
 instance asEmpValid_forall {α} [bi : BI PROP] (Φ : α → Prop) (P : α → PROP)
-  [hP : ∀ x, AsEmpValid d (Φ x) io PROP bi iprop(P x)]
-: AsEmpValid d (∀ x, Φ x) io PROP bi iprop(∀ x, P x) where
+    [hP : ∀ x, AsEmpValid d (Φ x) PROP bi iprop(P x)] :
+    AsEmpValid d (∀ x, Φ x) PROP bi iprop(∀ x, P x) where
   as_emp_valid := ⟨λ hd h => forall_intro λ x => (hP x).1.1 hd (h x),
                    λ hd h x => (hP x).1.2 hd $ h.trans (forall_elim x)⟩
 
